Lean4Lean/Theory/Typing/EnvLemmas.lean
@@ -1,0 +1,27 @@
+import Lean4Lean.Theory.Typing.Lemmas
+import Lean4Lean.Theory.Typing.Env
+import Lean4Lean.Theory.Typing.QuotLemmas
+import Lean4Lean.Theory.Typing.InductiveLemmas
+
+namespace Lean4Lean
+
+open Lean (Name FVarId)
+open VExpr
+
+theorem VEnv.WF.ordered (H : WF env ds) : Ordered env := by
+  induction H with
+  | empty => exact .empty
+  | decl h _ ih =>
+    cases h with
+    | block h => exact .const ih (by rintro _ ⟨⟩) h
+    | «axiom» h1 h2 => exact .const ih (by rintro _ ⟨⟩; exact h1) h2
+    | @«def» env env' ci h1 h2 =>
+      refine .defeq (.const ih (by rintro _ ⟨⟩; exact h1.isType ih ⟨⟩) h2) ⟨?_, ?_⟩
+      · simp [VDefVal.toDefEq]
+        rw [← (h1.levelWF ⟨⟩).2.2.instL_id]
+        exact .const (addConst_self h2) VLevel.id_WF (by simp)
+      · exact h1.mono (addConst_le h2)
+    | «opaque» h1 h2 => exact .const ih (by rintro _ ⟨⟩; exact h1.isType ih ⟨⟩) h2
+    | «example» _ => exact ih
+    | quot h1 h2 => exact addQuot_WF ih h1 h2
+    | induct h1 h2 => exact addInduct_WF ih h1 h2
