Lean4Lean/Theory/Typing/InductiveLemmas.lean
@@ -1,0 +1,14 @@
+import Std
+import Lean4Lean.Theory.Typing.Lemmas
+import Lean4Lean.Theory.Typing.Env
+
+namespace Lean4Lean
+
+open Lean (Name FVarId)
+open VExpr
+
+namespace VEnv
+
+theorem addInduct_WF (henv : Ordered env) (hdecl : decl.WF env)
+    (henv' : addInduct env decl = some env') : Ordered env' :=
+  sorry
