Lean4Lean/Theory/Typing/Meta.lean
@@ -1,0 +1,55 @@
+import Lean4Lean.Theory.Typing.Lemmas
+
+namespace Lean4Lean
+
+open Lean (Name FVarId)
+open VExpr
+
+namespace VEnv
+
+theorem with_addConst {P : Prop} {env env' : VEnv} {cis : List (Name × VConstant)}
+    (henv : Ordered env)
+    (hci : (cis.All fun ci => env.constants ci.1 = ci.2) → ci.WF env)
+    (IH : ∀ {env1}, Ordered env1 →
+      (((n, ci) :: cis).All fun ci => env1.constants ci.1 = ci.2) → f env1 = some env' → P)
+    (hcis : cis.All fun ci => env.constants ci.1 = ci.2)
+    (H : (env.addConst n (some ci) >>= f) = some env') : P := by
+  let ⟨env1, h1, henv1⟩ := Option.bind_eq_some.1 H
+  refine IH (.const henv (by rintro _ ⟨⟩; exact hci hcis) h1) ?_ henv1
+  exact ⟨addConst_self h1, hcis.imp fun _ => (addConst_le h1).1 _ _⟩
+
+theorem Lookup.zero' (eq : A.lift = ty') :
+    Lookup (A::Γ) 0 ty' := eq ▸ .zero
+theorem Lookup.succ' (h : Lookup Γ n ty) (eq : ty.lift = ty') :
+    Lookup (A::Γ) (n+1) ty' := eq ▸ .succ h
+
+syntax "lookup_tac" : tactic
+macro_rules | `(tactic| lookup_tac) => `(tactic|
+  first
+  | refine Lookup.zero' ?a (ty' := ?_); case a => exact rfl
+  | refine Lookup.succ' ?a ?b (ty := ?_) (ty' := ?_); (case a => lookup_tac); case b => exact rfl
+)
+
+theorem IsDefEq.app' (h1 : HasType env U Γ f (.forallE A B)) (h2 : HasType env U Γ a A)
+    (eq : B.inst a = B') : HasType env U Γ (.app f a) B' := eq ▸ .appDF h1 h2
+theorem IsDefEq.const'
+  (h1 : constants env c = some (some ci))
+  (h2 : ∀ (l : VLevel), l ∈ ls → VLevel.WF uvars l)
+  (h3 : List.length ls = ci.uvars)
+  (eq : .instL ls ci.type = ty') :
+  HasType env uvars Γ (.const c ls) ty' := eq ▸ .const h1 h2 h3
+
+syntax "type_tac" : tactic -- TODO: write an actual tactic
+macro_rules | `(tactic| type_tac) => `(tactic|
+  first
+  | refine IsDefEq.forallE ?a ?b (u := ?_) (v := ?_)
+    (case a => type_tac); (case b => type_tac)
+  | refine IsDefEq.sort ?a; (case a => decide)
+  | refine IsDefEq.bvar ?a; (case a => lookup_tac)
+  | refine IsDefEq.app' ?f ?a ?eq (A := ?_) (B := ?_)
+    (case f => type_tac); (case a => type_tac); (case eq => exact rfl)
+  | refine IsDefEq.const' ?h1 ?h2 ?h3 ?eq (ci := ?_)
+    (case h1 => assumption); (case h2 => decide); (case h3 => decide); (case eq => exact rfl)
+  | refine IsDefEq.lam ?h1 ?h2 (u := ?_)
+    (case h1 => type_tac); (case h2 => type_tac)
+)
