Lean4Lean/Theory/Typing/QuotLemmas.lean
@@ -1,0 +1,18 @@
+import Lean4Lean.Theory.Typing.Env
+import Lean4Lean.Theory.Typing.Meta
+
+namespace Lean4Lean
+
+open Lean (Name FVarId)
+open VExpr
+
+namespace VEnv
+
+theorem addQuot_WF (henv : Ordered env) (hq : QuotReady env) :
+    addQuot env = some env' → Ordered env' := by
+  refine with_addConst (cis := [(_, _)]) (hcis := ⟨hq, ⟨⟩⟩) henv
+    (fun _ => ⟨_, by type_tac⟩) fun henv => ?_
+  refine with_addConst henv (fun ⟨quot, _⟩ => ⟨_, by type_tac⟩) fun henv => ?_
+  refine with_addConst henv (fun ⟨_, quot, _⟩ => ⟨_, by type_tac⟩) fun henv => ?_
+  refine with_addConst henv (fun ⟨_, _, quot, eq, _⟩ => ⟨_, by type_tac⟩) fun henv => ?_
+  rintro ⟨_, _, _, _, eq, _⟩ ⟨⟩; exact .defeq henv ⟨by type_tac, by type_tac⟩
